\documentclass[class=cs245,leqno]{agony}
\title{Useful Proofs/Exercises}

\declaretheorem{theorem}[unnumbered]
\begin{document}
\thispagestyle{firstpage}
\tableofcontents

\section{Logic06}
\subsection{Theorems}
\begin{theorem}[Double Negation]
  \logic{A |-| !!A}
\end{theorem}
\begin{prf}
  In the forwards direction:
  \begin{deduce}
    \l1 !!A     |- !!A \j {Ref}           \\
    \l2 !!A, !A |- !!A \j {+, \r1}        \\
    \l3 !A      |- !A  \j {+}             \\
    \l4 !!A, !A |- !A  \j {+, \r3}        \\
    \l5 A       |- !!A \j {! -, \r2, \r4}
  \end{deduce}
  In the backwards direction:
  \begin{deduce}
    \l1 A, !A |- A   \j {\E}            \\
    \l2 A, !A |- !A  \j {\E}            \\
    \l3 A     |- !!A \j {! +, \r1, \r2}
  \end{deduce}
\end{prf}

\begin{theorem}[Inconsistency Rule]
  \logic{!A, A |- B}
\end{theorem}
\begin{prf}
  \begin{deduce}
    \l1 A, !A, !B |- A  \j {\E}            \\
    \l2 A, !A, !B |- !A \j {\E}            \\
    \l3 A, !A,    |- B  \j {! -, \r1, \r2}
  \end{deduce}
\end{prf}

\begin{theorem}[Disjunctive Syllogism]
  \logic{A or B, !A |- B}
\end{theorem}
\begin{prf}
  \begin{deduce}
    \l1 !A, B      |- B \j {\E}                 \\
    \l2 !A, A      |- B \j {Inconsistency Rule} \\
    \l3 !A, A or B |- B \j {or -, \r1, \r2}
  \end{deduce}
\end{prf}

\begin{theorem}[Modus Tollens]
  \logic{!B, A -> B |- !A}
\end{theorem}
\begin{prf}
  \begin{deduce}
    \l1 !B, !A or B |- !A     \j {Disjunctive Syllogism} \\
    \l2 !A or B     |- A -> B \j {Implication}           \\
    \l3 !B, A -> B  |- !A     \j {Repl., \r1, \r2}
  \end{deduce}
\end{prf}

\begin{theorem}[Contrapositive]
  \logic{A -> B |- !A -> !B}
\end{theorem}
\begin{prf}
  In the forwards direction:
  \begin{deduce}
    \l1 A -> B, !B |- !A       \j {Modus Tollens} \\
    \l2 A -> B     |- !B -> !A \j {-> +, \r1}
  \end{deduce}
  In the backwards direction:
  \begin{deduce}
    \l1 B or !A, !!A |- B      \j {Disjunctive Syllogism}       \\
    \l2 B or !A, A   |- B      \j {Repl., Double Negation, \r1} \\
    \l3 !!B or !A, A |- B      \j {Repl., Double Negation, \r2} \\
    \l4 !B -> !A, A  |- B      \j {Repl., Implication, \r3}     \\
    \l5 !B -> !A     |- A -> B \j {-> +, \r4}
  \end{deduce}
\end{prf}

\begin{theorem}[Affirmation]
  $A \d B$ if and only if $\0 \d A \i B$
\end{theorem}
\begin{prf}
  In the forwards direction:
  \begin{deduce}
    \l1 \0 |- A -> B \j {Premise}        \\
    \l3 A  |- A -> B \j {+, \r1}         \\
    \l2 A  |- A      \j {Ref}            \\
    \l4 A  |- B      \j {-> -, \r2, \r3}
  \end{deduce}
  The backwards direction is just (\i +) on the premise.
\end{prf}

\begin{theorem}[Flip-Flop]
  If \logic{A |- B}, then \logic{!B |- !A}.
\end{theorem}
\begin{prf}
  Suppose $A \d B$. Then,
  \begin{deduce}
    \l1 A  |- B        &  \j {Premise}                    \\
    \l2 \0 |- A -> B   &  \j {-> +, \r1}                  \\
    \l3 \0 |- !B -> !A &  \j {Repl., Contrapositive, \r2} \\
    \l4 !B |- !A       &  \j {Affirmation, \r3}
  \end{deduce}
  as desired.
\end{prf}

\begin{theorem}[De Morgan 1]
  \logic{!(A or B) |-| !A and !B}
\end{theorem}
\begin{prf}
  In the forwards direction:
  \begin{deduce}
    \l1 !(A or B), A |- A         \j {\E}              \\
    \l2 !(A or B), A |- A or B    \j {or +, \r1}       \\
    \l3 !(A or B), A |- !(A or B) \j {\E}              \\
    \l4 !(A or B)    |- !A        \j {! +, \r2, \r3}   \\
    \l5 !(A or B), B |- B         \j {\E}              \\
    \l6 !(A or B), B |- A or B    \j {or +, \r5}       \\
    \l7 !(A or B), B |- !(A or B) \j {\E}              \\
    \l8 !(A or B)    |- !B        \j {! +, \r6, \r7}   \\
    \l9 !(A or B)    |- !A and !B \j {and +, \r5, \r8}
  \end{deduce}
  Backwards:
  \begin{deduce}
    \l1 !A and !B, A or B |- A or B    \j {\E}                              \\
    \l2 !A and !B, A or B |- !A and !B \j {\E}                              \\
    \l3 !A and !B, A or B |- !A        \j {and -, \r2}                      \\
    \l4 !A and !B, A or B |- !B        \j {and -, \r2}                      \\
    \l5 !A and !B, A or B |- A         \j {Disjunctive Syllogism, \r1, \r4} \\
    \l6 !A and !B         |- !(A or B) \j {! +, \r3, \r5}
  \end{deduce}
\end{prf}

\begin{theorem}[De Morgan 2]
  \logic{!(A and B) |-| !A or !B}
\end{theorem}
\begin{prf}
  Forwards:
  \begin{deduce}
    \l1 !(A and B), !(!A or !B) |- !(!A or !B) \j {\E}                          \\
    \l2 !(A and B), !(!A or !B) |- !!A and !!B \j {Tr., De Morgan 1, \r1}       \\
    \l3 !(A and B), !(!A or !B) |- A and B     \j {Repl., Double Negation, \r2} \\
    \l4 !(A and B), !(!A or !B) |- !(A and B)  \j {\E}                          \\
    \l5 !(A and B)              |- !A or !B    \j {! -, \r3, \r4}
  \end{deduce}
  Backwards:
  \begin{deduce}
    \l1 !A or !B, A and B |- A and B    \j {\E}                              \\
    \l2 !A or !B, A and B |- A          \j {and -, \r1}                      \\
    \l3 !A or !B, A and B |- B          \j {and -, \r1}                      \\
    \l4 !A or !B, A and B |- !!B        \j {Double Negation, \r3}            \\
    \l5 !A or !B, A and B |- !A or !B   \j {\E}                              \\
    \l6 !A or !B, A and B |- !A         \j {Disjunctive Syllogism, \r5, \r4} \\
    \l7 !A or !B          |- !(A and B) \j {! +, \r2, \r6}
  \end{deduce}
\end{prf}

\begin{theorem}[Implication]
  \logic{A -> B |-| !A or B}
\end{theorem}
\begin{prf}
  Forwards:
  \begin{deduce}
    \l1 A -> B, !(!A or B) |- !(!A or B) \j {\E}                          \\
    \l8 A -> B, !(!A or B) |- !!A and !B \j {Tr., De Morgan 1, \r1}       \\
    \l2 A -> B, !(!A or B) |- A and !B   \j {Repl., Double Negation, \r8} \\
    \l3 A -> B, !(!A or B) |- A          \j {and -, \r2}                  \\
    \l4 A -> B, !(!A or B) |- A -> B     \j {\E}                          \\
    \l5 A -> B, !(!A or B) |- B          \j {-> -, \r4, \r3}              \\
    \l6 A -> B, !(!A or B) |- !B         \j {and -, \r2}                  \\
    \l7 A -> B             |- !A or B    \j {! -, \r5, \r6}
  \end{deduce}
  Backwards:
  \begin{deduce}
    \l1 !A or B, A |- A       \j {\E}                              \\
    \l2 !A or B, A |- !!A     \j {Double Negation, \r1}            \\
    \l3 !A or B, A |- !A or B \j {\E}                              \\
    \l4 !A or B, A |- B       \j {Disjunctive Syllogism, \r3, \r2} \\
    \l5 !A or B    |- A -> B  \j {-> +, \r4}
  \end{deduce}
\end{prf}

\begin{theorem}[Non-Contradiction]
  \logic{\0 |- !(A and !A)}
\end{theorem}
\begin{prf}
  \begin{deduce}
    \l0 A and !A |- A and !A    \j {Ref}             \\
    \l1 A and !A |- A           \j {Tr., and -, \r0} \\
    \l2 A and !A |- !A          \j {Tr., and -, \r0} \\
    \l3 \0       |- !(A and !A) \j {! +, \r1, \r2}
  \end{deduce}
\end{prf}

\begin{theorem}[Excluded Middle]
  \logic{\0 |- A or !A}
\end{theorem}
\begin{prf}
  Apply Transitivity, De Morgan 2 to Non-Contradiction.
\end{prf}

\begin{theorem}[Rule of Cases]
  \logic{A -> B, !A -> B |- B}
\end{theorem}
\begin{prf}
  \begin{deduce}
    \l1 A -> B, !A -> B, !B |- A -> B  \j {\E}                      \\
    \l2 A -> B, !A -> B, !B |- !A -> B \j {\E}                      \\
    \l3 A -> B, !A -> B, !B |- !B      \j {\E}                      \\
    \l4 A -> B, !A -> B, !B |- !A      \j {Modus Tollens, \r1, \r3} \\
    \l5 A -> B, !A -> B, !B |- !!A     \j {Modus Tollens, \r2, \r3} \\
    \l6 A -> B, !A -> B     |- B       \j {! -, \r4, \r5}
  \end{deduce}
\end{prf}

\subsection{Exercises}
\begin{xca}
  \logic{A -> (B or C), A -> !B, C -> !D |- A -> !D}
\end{xca}
\begin{prf}
  Let $\S = \logic{\{A -> (B or C), A -> !B, C -> !D\}}$.
  \begin{deduce}
    \l1 \S, A |- A             \j {\E}                              \\
    \l2 \S, A |- A -> (B or C) \j {\E}                              \\
    \l3 \S, A |- B or C        \j {-> -, \r2, \r1}                  \\
    \l4 \S, A |- A -> !B       \j {\E}                              \\
    \l5 \S, A |- !B            \j {-> -, \r4, \r1}                  \\
    \l6 \S, A |- C             \j {Disjunctive Syllogism, \r3, \r5} \\
    \l7 \S, A |- C -> !D       \j {\E}                              \\
    \l8 \S, A |- !D            \j {-> -, \r7, \r6}                  \\
    \l9 \S    |- A -> !D       \j {-> +, \r8}
  \end{deduce}
\end{prf}

\begin{xca}
  \logic{A -> (B -> C), C -> !D, !E -> D, A and B |- E}
\end{xca}
\begin{prf}
  Let $\S = \logic{\{A -> (B -> C), C -> !D, !E -> D, A and B\}}$.
  \begin{deduce}
    \l0 \S |- A and B       \j {\E}                      \\
    \l1 \S |- A             \j {and -, \r0}              \\
    \l2 \S |- A -> (B -> C) \j {\E}                      \\
    \l3 \S |- B -> C        \j {-> -, \r2, \r1}          \\
    \l4 \S |- B             \j {and -, \r0}              \\
    \l5 \S |- C             \j {-> -, \r3, \r4}          \\
    \l6 \S |- C -> !D       \j {\E}                      \\
    \l7 \S |- !D            \j {-> -, \r6, \r5}          \\
    \l8 \S |- !E -> D       \j {\E}                      \\
    \l9 \S |- E             \j {Modus Tollens, \r7, \r8}
  \end{deduce}
\end{prf}

\begin{xca}
  \logic{!A -> C or D, B -> E and F, E -> D, !D |- (A -> B) -> C}
\end{xca}
\begin{prf}
  Let $\S = \logic{!A -> C or D, B -> E and F, E -> D, !D}$
  \begin{deduce}
    \l 0 \S, A -> B |- E -> D        \j {\E}                               \\
    \l 1 \S, A -> B |- !D            \j {\E}                               \\
    \l 2 \S, A -> B |- !E            \j {Modus Tollens, \r1, \r0}          \\
    \l 3 \S, A -> B |- !E or !F      \j {or +, \r2}                        \\
    \l 4 \S, A -> B |- !(E and F)    \j {Tr., De Morgan, \r3}              \\
    \l 5 \S, A -> B |- B -> E and F  \j {\E}                               \\
    \l 6 \S, A -> B |- !B            \j {Modus Tollens, \r4, \r5}          \\
    \l 7 \S, A -> B |- A -> B        \j {\E}                               \\
    \l 8 \S, A -> B |- !A            \j {Modus Tollens, \r6, \r7}          \\
    \l 9 \S, A -> B |- !A -> C or D  \j {\E}                               \\
    \l a \S, A -> B |- C or D        \j {-> -, \r9}                        \\
    \l b \S, A -> B |- C             \j {Disjunctive Syllogism, \r a, \r1} \\
    \S              |- (A -> B) -> C \j {-> +, \r b}
  \end{deduce}
\end{prf}

\begin{xca}
  \logic{!(A or B) -> (C -> D), !A and !D |- !B -> !C}
\end{xca}
\begin{prf}
  Let $\S = \logic{!(A or B) -> (C -> D), !A and !D}$.
  \begin{deduce}
    \l 1 \S, !B |- !(A or B) -> (C -> D)   \j {\E}                      \\
    \l 2 \S, !B |- (!A and !B) -> (C -> D) \j {Repl., De Morgan, \r1}   \\
    \l 3 \S, !B |- !A and !D               \j {\E}                      \\
    \l 4 \S, !B |- !A                      \j {and -, \r3}              \\
    \l 5 \S, !B |- !B                      \j {\E}                      \\
    \l 6 \S, !B |- !A and !B               \j {and +, \r4, \r5}         \\
    \l 7 \S, !B |- C -> D                  \j {-> -, \r2, \r6}          \\
    \l 8 \S, !B |- !D                      \j {and -, \r3}              \\
    \l 9 \S, !B |- !C                      \j {Modus Tollens, \r8, \r7} \\
    \l a \S     |- !B -> !C                \j {-> +, \r9}
  \end{deduce}
\end{prf}

\begin{xca}
  \logic{B or A, B -> A |- !(A -> !A)}
\end{xca}
\begin{prf}
  Let $\S = \{\logic{B or A, B -> A}\}$
  \begin{deduce}
    \l 1 \S, A -> !A, !B |- !B         \j {\E}                              \\
    \l 2 \S, A -> !A, !B |- B or A     \j {\E}                              \\
    \l 3 \S, A -> !A, !B |- A          \j {Disjunctive Syllogism, \r1, \r2} \\
    \l 4 \S, A -> !A     |- !B -> A    \j {-> +, \r3}                       \\
    \l 5 \S, A -> !A     |- B -> A     \j {\E}                              \\
    \l 6 \S, A -> !A     |- A          \j {Tr., Rule of Cases, \r4, \r5}    \\
    \l 7 \S, A -> !A     |- A -> !A    \j {\E}                              \\
    \l 8 \S, A -> !A     |- !A         \j {-> -, \r7}                       \\
    \l 9 \S              |- !(A -> !A) \j {! +, \r6, \r8}
  \end{deduce}
\end{prf}


\section{Logic14}

\subsection{Exercises}

\begin{xca}
  \logic{\A[x]\A[y] P(x,y) |- \A[y]\A[x] P(x,y)}
\end{xca}
\begin{prf}
  \begin{deduce}
    \l1 \A[x]\A[y] P(x,y) |- \A[x]\A[y] P(x,y) \j {Ref}                          \\
    \l2 \A[x]\A[y] P(x,y) |- \A[y] P(a,y)      \j {\A -, \r1}                    \\
    \l3 \A[x]\A[y] P(x,y) |- P(a,b)            \j {\A -, \r2}                    \\
    \l4 \A[x]\A[y] P(x,y) |- \A[x] P(x,b)      \j {\A +, \r3, $a$ not elsewhere} \\
    \l5 \A[x]\A[y] P(x,y) |- \A[y] P(x,y)      \j {\A +, \r4, $b$ not elsewhere}
  \end{deduce}
\end{prf}

\begin{xca}
  \logic{\A[x] P(x) |- \A[y] P(y)}
\end{xca}
\begin{prf}
  \begin{deduce}
    \l1 \A[x] P(x) |- \A[x] P(x) \j {Ref}                          \\
    \l2 \A[x] P(x) |- P(a)       \j {\A -, \r1}                    \\
    \l3 \A[x] P(x) |- \A[y] P(y) \j {\A +, \r2, $a$ not elsewhere}
  \end{deduce}
\end{prf}

\begin{xca}
  \logic{!\X[x]P(x) |- \A[x]!P(x)}
\end{xca}
\begin{prf}
  \begin{deduce}
    \l1 \S, P(t) |- P(t)       \j {\E}                      \\
    \l2 \S, P(t) |- \X[x]P(x)  \j {\X +, \r1}               \\
    \l3 \S, P(t) |- !\X[x]P(x) \j {\E}                      \\
    \l4 \S       |- !P(t)      \j {! +, \r2, \r3}           \\
    \l5 \S       |- \A[x]!P(x) \j {\A +, $t$ not elsewhere}
  \end{deduce}
\end{prf}

\begin{xca}
  \logic{\A[x]!P(x) |- !\X[x]P(x)}
\end{xca}
\begin{prf}
  \begin{deduce}
    \l1 \S, \X[x]P(x), P(u) |- P(u)       \j {\E}                      \\
    \l2 \S, \X[x]P(x), P(u) |- \A[x]!P(x) \j {\E}                      \\
    \l3 \S, \X[x]P(x), P(u) |- !P(u)      \j {Tr., \A -, \r2}          \\
    \l4 \S, P(u)            |- !\X[x]P(x) \j {! +, \r1, \r3}           \\
    \l5 \S, \X[x]P(x)       |- !\X[x]P(x) \j {\X -, $u$ not elsewhere} \\
    \l6 \S, \X[x]P(x)       |- \X[x]P(x)  \j {\E}                      \\
    \l7 \S                  |- !\X[x]P(x) \j {! +, \r5, \r6}
  \end{deduce}
\end{prf}

\begin{xca}
  \logic{\A[x](P(x) -> Q(x)), \X[x](R(x) and !Q(x)), \A[x](R(x) -> P(x) or S(x)) |- \X[x](R(x) or S(x))}
\end{xca}
\begin{prf}
  Let $\logic{\S = \{\A[x](P(x) -> Q(x)), \A[x](R(x) -> P(x) or S(x))\}}$
  \begin{deduce}
    \l 0 \S, R(u) and !Q(u)        |- R(u) and !Q(u)              \j {\E}                              \\
    \l 1 \S, R(u) and !Q(u)        |- !Q(u)                       \j {and -, \r0}                      \\
    \l 2 \S, R(u) and !Q(u)        |- \A[x](P(x) -> Q(x))         \j {\E}                              \\
    \l 3 \S, R(u) and !Q(u)        |- P(u) -> Q(u)                \j {\A -, \r2}                       \\
    \l 4 \S, R(u) and !Q(u)        |- !P(u)                       \j {modus tollens, \r1, \r3}         \\
    \l 5 \S, R(u) and !Q(u)        |- \A[x](R(x) -> P(x) or S(x)) \j {\E}                              \\
    \l 6 \S, R(u) and !Q(u)        |- R(u) -> P(u) or S(u)        \j {\A -, \r5}                       \\
    \l 7 \S, R(u) and !Q(u)        |- R(u)                        \j {and -, \r0}                      \\
    \l 8 \S, R(u) and !Q(u)        |- P(u) or S(u)                \j {-> -, \r7, \r6}                  \\
    \l 9 \S, R(u) and !Q(u)        |- S(u)                        \j {Disjunctive Syllogism, \r8, \r4} \\
    \l a \S, R(u) and !Q(u)        |- R(u) or S(u)                \j {or +, \r7, \r9}                  \\
    \l b \S, R(u) and !Q(u)        |- \X[x](R(x) or S(x))         \j {\X +, \r a}                      \\
    \l c \S, \X[x](R(x) and !Q(x)) |- \X[x](R(x) or S(x))         \j {\X -, \r b, $u$ not elsewhere}
  \end{deduce}
\end{prf}

\end{document}